Modify a bit swap

theories/tests/swap.v
@@ -4,25 +4,29 @@ Section example.
   Context `{clangG Σ}.
 
   Definition x: ident := 1.
+  Definition a1: ident := 2.
+  Definition a2: ident := 3.
 
-  Definition Edecl (t: type) (x: ident) e : expr :=
-    Elet_typed t x (Ealloc t (Evalue (default_val t))) e.
+  Definition swap (t: type) :=
+    Edecl t x (
+    x <- a1 ;;
+    a1 <- a2 ;;
+    a2 <- x
+    ).
 
-  Definition swap (t: type) (l1 l2: addr) :=
-    Edecl t x
-    (x <- ! l1 @ t ;; l1 <- !l2 @ t ;; l2 <- x).
-
-  Lemma swap_spec t l1 l2 v1 v2 Φ :
-    l1 ↦ v1 @ t ∗ l2 ↦ v2 @ t ∗
-    (l1 ↦ v2 @ t -∗ l2 ↦ v1 @ t -∗ Φ void)
-    ⊢ WP swap t l1 l2 {{ Φ }}.
+  (* Instantiate the variables *)
+  Definition swap' t  (l1 l2: addr) :=
+    instantiate_let a1 l1 t (swap t) ≫= instantiate_let a2 l2 t.
+  
+  Lemma swap_spec' t swap_e l1 l2 v1 v2 :
+    swap' t l1 l2 = Some swap_e →
+    {{{ l1 ↦ v1 @ t ∗ l2 ↦ v2 @ t }}} swap_e {{{ RET void ; l1 ↦ v2 @ t ∗ l2 ↦ v1 @ t }}}.
   Proof.
-    iIntros "(Hl1 & Hl2 & HΦ)".
-    rewrite /swap /Edecl.
+    iIntros (??) "[Hl1 Hl2] HΦ". inversion H0.
     iDestruct (mapsto_typeof with "Hl1") as "%".
     iDestruct (mapsto_typeof with "Hl2") as "%".
     wp_alloc lx as "Hlx". wp_let.
-    wp_run. iApply ("HΦ" with "Hl1 Hl2").
+    wp_run. iApply ("HΦ" with "[Hl1 Hl2]"). iFrame.
   Qed.
 
 End example.
